notations

Given_Clause_Loops/Fair_DISCOUNT_Loop.thy
@@ -468,12 +468,12 @@ abbreviation Precprec_S :: "'f multiset \<Rightarrow> 'f multiset \<Rightarrow> 
 lemma wfP_Precprec_S: "wfP (\<prec>\<prec>S)"
   using minimal_element_def wfP_multp wf_Prec_S wfp_on_UNIV by blast
 
-definition \<mu>2 :: "('p, 'f) DLf_state \<Rightarrow> ('p, 'f) DLf_state \<Rightarrow> bool" where
-  "\<mu>2 St' St \<longleftrightarrow>
+definition Less_state :: "('p, 'f) DLf_state \<Rightarrow> ('p, 'f) DLf_state \<Rightarrow> bool" (infix "\<sqsubset>" 50) where
+  "St' \<sqsubset> St \<longleftrightarrow>
    (yy_of St' = None \<and> yy_of St \<noteq> None)
    \<or> ((yy_of St' = None \<longleftrightarrow> yy_of St = None) \<and> mset_of_fstate St' \<prec>\<prec>S mset_of_fstate St)"
 
-lemma wfP_\<mu>2: "wfP \<mu>2"
+lemma wfP_Less_state: "wfP (\<sqsubset>)"
 proof -
   let ?boolset = "{(b', b :: bool). b' < b}"
   let ?msetset = "{(M', M). M' \<prec>\<prec>S M}"
@@ -486,18 +486,19 @@ proof -
   have wf_lex_prod: "wf (?boolset <*lex*> ?msetset)"
     by (rule wf_lex_prod[OF wf_boolset wf_msetset])
 
-  have \<mu>2_alt_def: "\<And>St' St. \<mu>2 St' St \<longleftrightarrow> (?pair_of St', ?pair_of St) \<in> ?boolset <*lex*> ?msetset"
-    unfolding \<mu>2_def by auto
+  have Less_state_alt_def:
+    "\<And>St' St. St' \<sqsubset> St \<longleftrightarrow> (?pair_of St', ?pair_of St) \<in> ?boolset <*lex*> ?msetset"
+    unfolding Less_state_def by auto
 
   show ?thesis
-    unfolding wfP_def \<mu>2_alt_def using wf_app[of _ ?pair_of] wf_lex_prod by blast
+    unfolding wfP_def Less_state_alt_def using wf_app[of _ ?pair_of] wf_lex_prod by blast
 qed
 
-lemma non_compute_infer_choose_p_DLf_step_imp_\<mu>2:
+lemma non_compute_infer_choose_p_DLf_step_imp_Less_state:
   assumes
     step: "St \<leadsto>DLf St'" and
     yy: "yy_of St \<noteq> None \<or> yy_of St' = None"
-  shows "\<mu>2 St' St"
+  shows "St' \<sqsubset> St"
   using step
 proof cases
   case (compute_infer P \<iota> A C)
@@ -517,7 +518,7 @@ next
   case (delete_fwd C A P)
   note defs = this(1,2)
   show ?thesis
-    unfolding defs \<mu>2_def by (auto intro!: subset_implies_multp)
+    unfolding defs Less_state_def by (auto intro!: subset_implies_multp)
 next
   case (simplify_fwd C' C A P)
   note defs = this(1,2) and prec = this(3)
@@ -534,12 +535,13 @@ next
       unfolding multp_def using prec by (auto intro: singletons_in_mult)
   qed
   thus ?thesis
-    unfolding defs \<mu>2_def by simp
+    unfolding defs Less_state_def by simp
 next
   case (delete_bwd C' A C P)
   note defs = this(1,2) and c_ni = this(3)
   show ?thesis
-    unfolding defs \<mu>2_def using c_ni by (auto simp: fmember.rep_eq intro!: subset_implies_multp)
+    unfolding defs Less_state_def using c_ni
+    by (auto simp: fmember.rep_eq intro!: subset_implies_multp)
 next
   case (simplify_bwd C' A C'' C P)
   note defs = this(1,2) and c'_ni = this(3) and prec = this(4)
@@ -548,7 +550,7 @@ next
   proof (cases "C'' \<in> passive_formulas_of P")
     case c''_in: True
     show ?thesis
-      unfolding defs \<mu>2_def using c'_ni
+      unfolding defs Less_state_def using c'_ni
       by (auto simp: fmember.rep_eq insert_absorb[OF c''_in] intro!: subset_implies_multp)
   next
     case c''_ni: False
@@ -574,13 +576,13 @@ next
         unfolding multp_def using prec by (auto intro: singletons_in_mult)
     qed
     show ?thesis
-      unfolding defs \<mu>2_def by simp (simp only: bef aft lt_new)
+      unfolding defs Less_state_def by simp (simp only: bef aft lt_new)
   qed
 next
   case (schedule_infer \<iota>s A C P)
   note defs = this(1,2)
   show ?thesis
-    unfolding defs \<mu>2_def by auto
+    unfolding defs Less_state_def by auto
 next
   case (delete_orphan_infers \<iota>s P A Y)
   note defs = this(1,2) and \<iota>s_nnil = this(3) and \<iota>s_sub = this(4) and \<iota>s_inter = this(5)
@@ -590,20 +592,20 @@ next
         finite_passive_inferences_of finite_subset image_mset_subset_mono mset_set_eq_iff set_empty
         subset_imp_msubset_mset_set subset_mset.nless_le)
   thus ?thesis
-    unfolding defs \<mu>2_def by (auto intro!: subset_implies_multp)
+    unfolding defs Less_state_def by (auto intro!: subset_implies_multp)
 qed
 
-lemma yy_nonempty_DLf_step_imp_\<mu>2:
+lemma yy_nonempty_DLf_step_imp_Less_state:
   assumes
     step: "St \<leadsto>DLf St'" and
     yy: "yy_of St \<noteq> None" and
     yy': "yy_of St' \<noteq> None"
-  shows "\<mu>2 St' St"
+  shows "St' \<sqsubset> St"
 proof -
   have "yy_of St \<noteq> None \<or> yy_of St' = None"
     using yy by blast
   thus ?thesis
-    using non_compute_infer_choose_p_DLf_step_imp_\<mu>2[OF step] by blast
+    using non_compute_infer_choose_p_DLf_step_imp_Less_state[OF step] by blast
 qed
 
 lemma fair_DL_Liminf_yy_empty:
@@ -637,18 +639,19 @@ proof (rule ccontr)
     using full_chain_imp_chain[OF full] infinite_chain_lnth_rel len llength_eq_infty_conv_lfinite
     by blast
 
-  have "\<mu>2 (lnth Sts (Suc j)) (lnth Sts j)" if j_ge: "j \<ge> i" for j
-    using yy_nonempty_DLf_step_imp_\<mu>2 by (meson step j_ge yy_j yy_sj)
-  hence "\<mu>2\<inverse>\<inverse> (lnth Sts j) (lnth Sts (Suc j))" if j_ge: "j \<ge> i" for j
+  have "lnth Sts (Suc j) \<sqsubset> lnth Sts j" if j_ge: "j \<ge> i" for j
+    using yy_nonempty_DLf_step_imp_Less_state by (meson step j_ge yy_j yy_sj)
+  hence "(\<sqsubset>)\<inverse>\<inverse> (lnth Sts j) (lnth Sts (Suc j))" if j_ge: "j \<ge> i" for j
     using j_ge by blast
-  hence inf_down_chain: "chain \<mu>2\<inverse>\<inverse> (ldropn i Sts)"
+  hence inf_down_chain: "chain (\<sqsubset>)\<inverse>\<inverse> (ldropn i Sts)"
     by (simp add: chain_ldropnI si_lt)
 
   have inf_i: "\<not> lfinite (ldropn i Sts)"
     using len by (simp add: llength_eq_infty_conv_lfinite)
 
   show False
-    using inf_i inf_down_chain wfP_iff_no_infinite_down_chain_llist[of \<mu>2] wfP_\<mu>2 by metis
+    using inf_i inf_down_chain wfP_iff_no_infinite_down_chain_llist[of "(\<sqsubset>)"] wfP_Less_state
+    by metis
 qed
 
 lemma DLf_step_imp_queue_step:
@@ -702,18 +705,19 @@ proof -
         by blast
     qed auto
 
-    have "\<mu>2 (lnth Sts (Suc j)) (lnth Sts j)" if j_ge: "j \<ge> i" for j
-      by (rule non_compute_infer_choose_p_DLf_step_imp_\<mu>2[OF step[OF j_ge] yy[OF j_ge]])
-    hence "\<mu>2\<inverse>\<inverse> (lnth Sts j) (lnth Sts (Suc j))" if j_ge: "j \<ge> i" for j
+    have "lnth Sts (Suc j) \<sqsubset> lnth Sts j" if j_ge: "j \<ge> i" for j
+      by (rule non_compute_infer_choose_p_DLf_step_imp_Less_state[OF step[OF j_ge] yy[OF j_ge]])
+    hence "(\<sqsubset>)\<inverse>\<inverse> (lnth Sts j) (lnth Sts (Suc j))" if j_ge: "j \<ge> i" for j
       using j_ge by blast
-    hence inf_down_chain: "chain \<mu>2\<inverse>\<inverse> (ldropn i Sts)"
+    hence inf_down_chain: "chain (\<sqsubset>)\<inverse>\<inverse> (ldropn i Sts)"
       using chain_ldropn_lmapI[OF _ si_lt, of _ id, simplified llist.map_id] by simp
 
     have inf_i: "\<not> lfinite (ldropn i Sts)"
       using len lfinite_ldropn llength_eq_infty_conv_lfinite by blast
 
     show False
-      using inf_i inf_down_chain wfP_iff_no_infinite_down_chain_llist[of \<mu>2] wfP_\<mu>2 by blast
+      using inf_i inf_down_chain wfP_iff_no_infinite_down_chain_llist[of "(\<sqsubset>)"] wfP_Less_state
+      by blast
   qed
 
   have hd_emp: "lhd (lmap passive_of Sts) = empty"
